inductive case proved?

dp/edit_dist.dfy
@@ -1,14 +1,4 @@
-include "../authoring/seq.dfy"
-
 module EditDistance {
-    import Seq = Seq
-
-    function popChar(i: int): int
-    requires i >= 0
-    {
-        if i-1 < 0 then 0 else i-1 
-    }
-
     function diff(a: char, b: char): int
     {
         if a == b then 0 else 1
@@ -17,102 +7,55 @@ module EditDistance {
     function recEdDist(a: string, b: string): int
     requires |a| > 0 && |b| > 0
     {
-        0
-    }
-
-    function case1(a: string, b: string, ai: nat, bi: nat): int
-    requires 0 < ai+1 < |a|
-    requires 0 < bi+1 < |b|
-    decreases |a|- ai
-    {
-        1 + recEdDist'(a, b, ai+1, bi)
-    }
-
-    function case2(a: string, b: string, ai: nat, bi: nat): int
-    requires 0 < ai+1 < |a|
-    requires 0 < bi+1 < |b|
-    decreases |b| - bi
-    {
-        1 + recEdDist'(a, b, ai, bi+1)
-    }
-
-    function case3(a: string, b: string, ai: nat, bi: nat): int
-    requires 0 < ai+1 < |a|
-    requires 0 < bi+1 < |b|
-    decreases |a|- ai, |b| - bi
-    {
-        diff(a[ai], b[bi]) + recEdDist'(a, b, ai+1, bi+1)
+        recEdDist'(a, b, 0, 0)
     }
 
     function recEdDist'(a: string, b: string, ai: nat, bi: nat): int
-    requires 0 <= ai < |a|
-    requires 0 <= bi < |b|
-    decreases |a|- ai, |b| - bi
+    requires 0 <= ai <= |a|
+    requires 0 <= bi <= |b|
+    decreases |a|-ai, |b|-bi
     {
         // Both strings are empty, nothing to edit.
-        if ai+1 == |a| && bi+1 == |b| then 0 else
+        if ai == |a| && bi == |b| then 0 else
 
         /* If `a` is empty but not `b`, we need to
          * edit the remaining characters including
          * the character at index `bi`.
          */
-        if ai+1 == |a| then |b[bi..]| else
-        if bi+1 == |b| then |a[ai..]| else
-        if case1(a, b, ai, bi) < case2(a, b, ai, bi) 
-            && case1(a, b, ai, bi) < case3(a, b, ai, bi)
-        then case1(a, b, ai, bi) else
-        if case2(a, b, ai, bi) < case1(a, b, ai, bi) 
-            && case2(a, b, ai, bi) < case3(a, b, ai, bi)
-        then case2(a, b, ai, bi) else
-        case3(a, b, ai, bi)
+        if ai == |a| then |b[bi..]| else
+        if bi == |b| then |a[ai..]| else
+
+        // There's gotta be a better way.
+        if 1 + recEdDist'(a, b, ai+1, bi) < 1 + recEdDist'(a, b, ai, bi+1) 
+            && 1 + recEdDist'(a, b, ai+1, bi) < diff(a[ai], b[bi]) + recEdDist'(a, b, ai+1, bi+1)
+        then 1 + recEdDist'(a, b, ai+1, bi) else
+        if 1 + recEdDist'(a, b, ai, bi+1) < 1 + recEdDist'(a, b, ai+1, bi) 
+            && 1 + recEdDist'(a, b, ai, bi+1) < diff(a[ai], b[bi]) + recEdDist'(a, b, ai+1, bi+1)
+        then 1 + recEdDist'(a, b, ai, bi+1) else
+        diff(a[ai], b[bi]) + recEdDist'(a, b, ai+1, bi+1)
     }
-
-
-    lemma editDist(a: string, b: string, ai: int, bi: int) returns (dist: int)
-    requires |a| > 0 && |b| > 0
-    requires 0 <= ai < |a|
-    requires 0 <= bi < |b|
-    decreases ai, bi
-    {
-        var case1, case2, case3 :int;
-
-        if ai-1 < 0 {
-            case1 := 0;
-        } else {
-            case1 := editDist(a, b, ai-1, bi);
-            case1 := 1 + case1;
-        }
-
-        if bi-1 < 0 {
-            case2 := 0;
-        } else {
-            case2 := editDist(a, b, ai, bi-1);
-            case2 := 1 + case2;
-        }
-
-        if ai-1 < 0 || bi-1 < 0 {
-            case3 := 0;
-        } else {
-            case3 :=  editDist(a, b, ai-1, bi-1);
-            case3 := diff(a[ai], b[bi]) + case3;
-        }
-
-
-        var res :seq<int> := [case1, case2 , case3];
-        dist := Seq.calcMin(res);
-    }
-
 
     method Main()
     {
         var s1 := "a";
+        assert |s1| == 1;
+
         var s2 := "a";
         var s3 := "b";
+        var s4 := "snowy";
+        var s5 := "sunny";
+        var s6 := "aa";
+        var s7 := "aa";
 
         // Base case: both characters are the same, so no editing cost.
         assert recEdDist(s1, s2) == 0;
 
         // Base case: character substitution. 
         assert recEdDist(s1, s3) == 1;
+        
+        // Inductive:
+        assert recEdDist(s4, s5) == 3;
+
+        assert recEdDist(s6, s7) == 0;
     }
 }
